src/lowparse/LowParse.Low.VCList.fst
@@ -10,7 +10,7 @@ module B = LowStar.Buffer
 
 let valid_nlist_nil
   (#k: parser_kind)
-  (#t: Type0)
+  (#t: Type)
   (p: parser k t)
   (h: HS.mem)
   (#rrel #rel: _)
@@ -24,7 +24,7 @@ let valid_nlist_nil
 
 let valid_nlist_nil_recip
   (#k: parser_kind)
-  (#t: Type0)
+  (#t: Type)
   (p: parser k t)
   (h: HS.mem)
   (#rrel #rel: _)
@@ -41,7 +41,7 @@ let valid_nlist_nil_recip
 let valid_nlist_cons
   (n: nat)
   (#k: parser_kind)
-  (#t: Type0)
+  (#t: Type)
   (p: parser k t)
   (h: HS.mem)
   (#rrel #rel: _)
@@ -73,7 +73,7 @@ let valid_nlist_cons
 let valid_nlist_cons_recip
   (n: nat)
   (#k: parser_kind)
-  (#t: Type0)
+  (#t: Type)
   (p: parser k t)
   (h: HS.mem)
   (#rrel #rel: _)
@@ -107,7 +107,7 @@ let valid_nlist_cons_recip
 let valid_nlist_cons'
   (n: nat)
   (#k: parser_kind)
-  (#t: Type0)
+  (#t: Type)
   (p: parser k t)
   (h: HS.mem)
   (#rrel #rel: _)
@@ -129,7 +129,7 @@ let valid_nlist_cons'
 let valid_nlist_cons_not
   (n: nat)
   (#k: parser_kind)
-  (#t: Type0)
+  (#t: Type)
   (p: parser k t)
   (h: HS.mem)
   (#rrel #rel: _)
@@ -152,7 +152,7 @@ inline_for_extraction
 let validate_nlist
   (n: U32.t)
   (#k: parser_kind)
-  (#t: Type0)
+  (#t: Type)
   (#p: parser k t)
   (v: validator p)
 : Tot (validator (parse_nlist (U32.v n) p))
@@ -210,7 +210,7 @@ inline_for_extraction
 let jump_nlist
   (n: U32.t)
   (#k: parser_kind)
-  (#t: Type0)
+  (#t: Type)
   (#p: parser k t)
   (v: jumper p)
 : Tot (jumper (parse_nlist (U32.v n) p))
@@ -260,7 +260,7 @@ let jump_nlist
 let rec valid_nlist_valid_list
   (n: nat)
   (#k: parser_kind)
-  (#t: Type0)
+  (#t: Type)
   (p: parser k t)
   (h: HS.mem)
   (#rrel #rel: _)
@@ -291,7 +291,7 @@ let rec valid_nlist_valid_list
 
 let rec valid_list_valid_nlist
   (#k: parser_kind)
-  (#t: Type0)
+  (#t: Type)
   (p: parser k t)
   (h: HS.mem)
   (#rrel #rel: _)
@@ -331,7 +331,7 @@ let validate_vclist
   (lv: validator lp)
   (lr: leaf_reader lp)
   (#k: parser_kind)
-  (#t: Type0)
+  (#t: Type)
   (#p: parser k t)
   (v: validator p)
 : Tot (validator (parse_vclist (U32.v min) (U32.v max) lp p))
@@ -363,7 +363,7 @@ let jump_vclist
   (lv: jumper lp)
   (lr: leaf_reader lp)
   (#k: parser_kind)
-  (#t: Type0)
+  (#t: Type)
   (#p: parser k t)
   (v: jumper p)
 : Tot (jumper (parse_vclist min max lp p))
@@ -388,7 +388,7 @@ let valid_vclist_elim
   (#lk: parser_kind)
   (lp: parser lk U32.t { lk.parser_kind_subkind == Some ParserStrong })
   (#k: parser_kind)
-  (#t: Type0)
+  (#t: Type)
   (p: parser k t)
   (h: HS.mem)
   (#rrel #rel: _)
@@ -418,7 +418,7 @@ let valid_vclist_intro
   (#lk: parser_kind)
   (lp: parser lk U32.t { lk.parser_kind_subkind == Some ParserStrong })
   (#k: parser_kind)
-  (#t: Type0)
+  (#t: Type)
   (p: parser k t)
   (h: HS.mem)
   (#rrel #rel: _)
