src/lowparse/LowParse.Spec.Fuel.fst
@@ -3,21 +3,21 @@ include LowParse.Spec.Base
 
 module Seq = FStar.Seq
 
-let injective_fuel (fuel: nat) (#t: Type0) (p: bare_parser t) : GTot Type0 =
+let injective_fuel (fuel: nat) (#t: Type) (p: bare_parser t) : GTot Type0 =
   forall (b1 b2: bytes) . {:pattern (injective_precond p b1 b2) \/ (injective_postcond p b1 b2)}
   (injective_precond p b1 b2 /\ Seq.length b1 < fuel /\ Seq.length b2 < fuel) ==>
   injective_postcond p b1 b2
 
 let no_lookahead_fuel
   (fuel: nat)
-  (#t: Type0)
+  (#t: Type)
   (f: bare_parser t)
 : GTot Type0
 = forall (x x' : bytes) . {:pattern (no_lookahead_on_precond f x x') \/ (no_lookahead_on_postcond f x x')} (Seq.length x < fuel /\ Seq.length x' < fuel) ==> no_lookahead_on f x x'
 
 let consumes_all_fuel
   (fuel: nat)
-  (#t: Type0)
+  (#t: Type)
   (p: bare_parser t)
 : GTot Type0
 = forall (b: bytes { Seq.length b < fuel }) . {:pattern (parse p b)} Some? (parse p b) ==> (
@@ -25,7 +25,7 @@ let consumes_all_fuel
     Seq.length b == len
   )
 
-let parser_subkind_prop_fuel (fuel: nat) (k: parser_subkind) (#t: Type0) (f: bare_parser t) : GTot Type0 =
+let parser_subkind_prop_fuel (fuel: nat) (k: parser_subkind) (#t: Type) (f: bare_parser t) : GTot Type0 =
   match k with
   | ParserStrong ->
     no_lookahead_fuel fuel f
@@ -35,7 +35,7 @@ let parser_subkind_prop_fuel (fuel: nat) (k: parser_subkind) (#t: Type0) (f: bar
 let parses_at_least_fuel
   (fuel: nat)
   (sz: nat)
-  (#t: Type0)
+  (#t: Type)
   (f: bare_parser t)
 : GTot Type0
 = forall (s: bytes { Seq.length s < fuel }) . {:pattern (parse f s)}
@@ -47,7 +47,7 @@ let parses_at_least_fuel
 let parses_at_most_fuel
   (fuel: nat)
   (sz: nat)
-  (#t: Type0)
+  (#t: Type)
   (f: bare_parser t)
 : GTot Type0
 = forall (s: bytes { Seq.length s < fuel }) . {:pattern (parse f s)}
@@ -59,22 +59,22 @@ let parses_at_most_fuel
 let is_total_constant_size_parser_fuel
   (fuel: nat)
   (sz: nat)
-  (#t: Type0)
+  (#t: Type)
   (f: bare_parser t)
 : GTot Type0
 = forall (s: bytes { Seq.length s < fuel }) . {:pattern (parse f s) }
   (Seq.length s < sz) == (None? (parse f s))
 
-let parser_always_fails_fuel (fuel: nat) (#t: Type0) (f: bare_parser t) : GTot Type0 =
+let parser_always_fails_fuel (fuel: nat) (#t: Type) (f: bare_parser t) : GTot Type0 =
   forall (input: bytes { Seq.length input < fuel }) . {:pattern (parse f input)} parse f input == None
 
-let parser_kind_metadata_prop_fuel (fuel: nat) (#t: Type0) (k: parser_kind) (f: bare_parser t) : GTot Type0 =
+let parser_kind_metadata_prop_fuel (fuel: nat) (#t: Type) (k: parser_kind) (f: bare_parser t) : GTot Type0 =
   match k.parser_kind_metadata with
   | None -> True
   | Some ParserKindMetadataTotal -> k.parser_kind_high == Some k.parser_kind_low ==> is_total_constant_size_parser_fuel fuel k.parser_kind_low f
   | Some ParserKindMetadataFail -> parser_always_fails_fuel fuel f
 
-let parser_kind_prop_fuel (fuel: nat) (#t: Type0) (k: parser_kind) (f: bare_parser t) : GTot Type0 =
+let parser_kind_prop_fuel (fuel: nat) (#t: Type) (k: parser_kind) (f: bare_parser t) : GTot Type0 =
   injective_fuel fuel f /\
   (Some? k.parser_kind_subkind ==> parser_subkind_prop_fuel fuel (Some?.v k.parser_kind_subkind) f) /\
   parses_at_least_fuel fuel k.parser_kind_low f /\
@@ -82,7 +82,7 @@ let parser_kind_prop_fuel (fuel: nat) (#t: Type0) (k: parser_kind) (f: bare_pars
   parser_kind_metadata_prop_fuel fuel k f
 
 unfold
-let parser_kind_prop' (#t: Type0) (k: parser_kind) (f: bare_parser t) : GTot Type0 =
+let parser_kind_prop' (#t: Type) (k: parser_kind) (f: bare_parser t) : GTot Type0 =
   injective f /\
   (Some? k.parser_kind_subkind ==> parser_subkind_prop (Some?.v k.parser_kind_subkind) f) /\
   parses_at_least k.parser_kind_low f /\
@@ -90,7 +90,7 @@ let parser_kind_prop' (#t: Type0) (k: parser_kind) (f: bare_parser t) : GTot Typ
   parser_kind_metadata_prop k f
 
 let injective_fuel_correct
-  (#t: Type0) (f: bare_parser t)
+  (#t: Type) (f: bare_parser t)
 : Lemma
   (requires (forall fuel . injective_fuel fuel f))
   (ensures (injective f))
@@ -98,7 +98,7 @@ let injective_fuel_correct
 
 let parses_at_least_fuel_correct
   (sz: nat)
-  (#t: Type0)
+  (#t: Type)
   (f: bare_parser t)
 : Lemma
   (requires (forall fuel . parses_at_least_fuel fuel sz f))
@@ -107,7 +107,7 @@ let parses_at_least_fuel_correct
 
 let parses_at_most_fuel_correct
   (sz: nat)
-  (#t: Type0)
+  (#t: Type)
   (f: bare_parser t)
 : Lemma
   (requires (forall fuel . parses_at_most_fuel fuel sz f))
@@ -115,7 +115,7 @@ let parses_at_most_fuel_correct
 = assert (forall x . Some? (parse f x) ==> parses_at_most_fuel (Seq.length x + 1) sz f)
 
 let parser_subkind_prop_fuel_correct
-  (k: parser_subkind) (#t: Type0) (f: bare_parser t)
+  (k: parser_subkind) (#t: Type) (f: bare_parser t)
 : Lemma
   (requires (forall fuel . parser_subkind_prop_fuel fuel k f))
   (ensures (parser_subkind_prop k f))
@@ -123,14 +123,14 @@ let parser_subkind_prop_fuel_correct
   assert (forall x . Some? (parse f x) ==> parser_subkind_prop_fuel (Seq.length x + 1) k f)
 
 let parser_kind_metadata_prop_fuel_correct
-  (#t: Type0) (k: parser_kind) (f: bare_parser t)
+  (#t: Type) (k: parser_kind) (f: bare_parser t)
 : Lemma
   (requires (forall fuel . parser_kind_metadata_prop_fuel fuel k f))
   (ensures (parser_kind_metadata_prop k f))
 = assert (forall x . let p =  (parse f x) in parser_kind_metadata_prop_fuel (Seq.length x + 1) k f)
 
 let parser_kind_prop_fuel_correct
-  (#t: Type0) (k: parser_kind) (f: bare_parser t)
+  (#t: Type) (k: parser_kind) (f: bare_parser t)
 : Lemma
   (requires (forall fuel . parser_kind_prop_fuel fuel k f))
   (ensures (parser_kind_prop' k f))
@@ -147,14 +147,14 @@ let parser_kind_prop_fuel_correct
   parser_kind_metadata_prop_fuel_correct k f
 
 let parser_kind_prop_fuel_complete'
-  (fuel: nat) (#t: Type0) (k: parser_kind) (f: bare_parser t)
+  (fuel: nat) (#t: Type) (k: parser_kind) (f: bare_parser t)
 : Lemma
   (requires (parser_kind_prop' k f))
   (ensures (parser_kind_prop_fuel fuel k f))
 = ()
 
 let parser_kind_prop_fuel_complete
-  (fuel: nat) (#t: Type0) (k: parser_kind) (f: bare_parser t)
+  (fuel: nat) (#t: Type) (k: parser_kind) (f: bare_parser t)
 : Lemma
   (requires (parser_kind_prop k f))
   (ensures (parser_kind_prop_fuel fuel k f))
@@ -162,7 +162,7 @@ let parser_kind_prop_fuel_complete
 
 let no_lookahead_fuel_ext
   (fuel: nat)
-  (#t: Type0)
+  (#t: Type)
   (p1 p2: bare_parser t)
 : Lemma
   (requires (
@@ -175,7 +175,7 @@ let no_lookahead_fuel_ext
 
 let injective_fuel_ext
   (fuel: nat)
-  (#t: Type0)
+  (#t: Type)
   (p1 p2: bare_parser t)
 : Lemma
   (requires (
@@ -189,7 +189,7 @@ let injective_fuel_ext
 
 let parser_kind_prop_fuel_ext
   (fuel: nat)
-  (#t: Type0)
+  (#t: Type)
   (k: parser_kind)
   (f1 f2: bare_parser t)
 : Lemma
@@ -199,14 +199,14 @@ let parser_kind_prop_fuel_ext
   injective_fuel_ext fuel f1 f2
 
 let close_by_fuel
-  (#t: Type0)
+  (#t: Type)
   (f: (nat -> Tot (bare_parser t)))
   (closure: ((b: bytes) -> GTot (n: nat { Seq.length b < n })))
 : Tot (bare_parser t)
 = fun x -> f (closure x) x
 
 let close_by_fuel_correct
-  (#t: Type0)
+  (#t: Type)
   (k: parser_kind)
   (f: (nat -> Tot (bare_parser t)))
   (closure: ((b: bytes) -> GTot (n: nat { Seq.length b < n })))
