src/lowparse/LowParse.Spec.VCList.fst
@@ -12,7 +12,7 @@ module L = FStar.List.Tot
 let parse_nlist
   (n: nat)
   (#k: parser_kind)
-  (#t: Type0)
+  (#t: Type)
   (p: parser k t)
 : Tot (y: parser (parse_nlist_kind n k) (nlist n t) { y == parse_nlist' n p } )
 = parse_nlist' n p
@@ -20,7 +20,7 @@ let parse_nlist
 let serialize_nlist
   (n: nat)
   (#k: parser_kind)
-  (#t: Type0)
+  (#t: Type)
   (#p: parser k t)
   (s: serializer p { k.parser_kind_subkind == Some ParserStrong } )
 : Tot (y: serializer (parse_nlist n p) { y == serialize_nlist' n s })
